---
title: | 
  | Phil/LPS 31 Introduction to Inductive Logic
  | Lecture 2
author: |
    | David Mwakima
    | dmwakima@uci.edu
    | University of California, Irvine
date: "April 5th 2023"
output: beamer_presentation
header-includes:
  - \setbeamertemplate{footline}[page number]
---

# Topics

\begin{itemize}
\item Sentential Logic: Formulas

\item Sentential Logic: Main connectives

\item Sentential Logic: Paraphrasing English

\item Truth tables

\item Truth functional equivalence
\end{itemize}

# Sentential Logic: Formulas

Remember that the \textcolor{red}{formal symbols} of sentential logic are:
\begin{enumerate} \item \textcolor{red}{$p$}, \textcolor{red}{$q$}, \textcolor{red}{$r$}, \textcolor{red}{$s$} and \textcolor{red}{$t$} as symbols for sentences. If we need more than 5 symbols (rarely!), then add the following countably many symbols \textcolor{red}{$p_{1}$}, \textcolor{red}{$p_{2}$}, \textcolor{red}{$p_{3}$}, \dots.
\item \textcolor{red}{$\vee$} for "or", \textcolor{red}{$\lnot$} for "not" since the other symbols for "and" and "if..., then..." can be defined from these. (More of this later)
\item \textcolor{red}{$($} for left bracket and \textcolor{red}{$)$} for right bracket.
\end{enumerate}

The \textcolor{red}{transformation rules} (also known as "syntactic rules") are:
\begin{enumerate}
\item Any sentence \textcolor{red}{$p$} is a formula.
\item If \textcolor{red}{$p$} is a formula, then \textcolor{red}{$\lnot p$} is formula.
\item If \textcolor{red}{$p$} is a formula and \textcolor{red}{$q$} is a formula, then \textcolor{red}{$(p \vee q)$} is a formula.
\end{enumerate}

The \textcolor{red}{closure condition} simply states that nothing else is a formula of sentential logic.

# Sentential Logic: Formulas

Are the following formulas in sentential logic? \begin{enumerate} \item $q$ \item $t$ \item $\lnot q$ \item $\lnot \lnot r$ \item $(\lnot \lnot \lnot p \vee q)$ \item $(p \vee (r \vee \lnot q))$ \item $((q \vee (t \vee s)) \vee (r \vee \lnot p))$ \end{enumerate}

# Sentential Logic: Formulas

Are the following formulas in sentential logic? \begin{enumerate} \item $a$ \item $b$ \item $q \lnot$ \item $\lnot r \lnot$ \item $(\lnot \vee \lnot p \vee q)$ \item $p \vee (r \vee \lnot q)$ \item $((q \vee (t \vee s)) \vee r \vee \lnot p)$ \end{enumerate}


# Sentential Logic: Main Connectives

>- Consider: \begin{enumerate} \item $((q \vee (t \vee s)) \vee (r \vee \lnot p))$ \item $((q \vee (t \vee s)) \vee r \vee \lnot p)$ \end{enumerate}

>- We said that (1) is a formula while (2) is not because \textcolor{red}{brackets matter}.

>- Think about similar uses of brackets in algebra. Brackets tell us which operations to do first. \begin{enumerate} \item $((24 \div 2) + 2) - 4 = 10$ 
\item $(24 \div (2 + 2)) - 4 = 2$ \end{enumerate}

>- So using brackets is not just a stipulation of our logic, it turns out that having brackets helps us \textcolor{red}{parse} the formula correctly in order to identify the \textcolor{red}{main connective}. In (1) we can identify the main connective but in (2) we cannot. This is why brackets matter.

# Sentential Logic: Main Connectives

>- We identified the main connective in (1) by thinking about how the formula was built up from simpler formulas. 

>- The main connective is the connective that is added last when forming complex formulas from simple ones and closing everything up with brackets.

>- Identify the main connective in these formulas: \begin{enumerate}
\item $\lnot q$ 
\item $\lnot \lnot r$ 
\item $(\lnot \lnot \lnot p \vee q)$ 
\item $(p \vee (r \vee \lnot q))$
\end{enumerate}


# Sentential Logic: Paraphrasing English



















